tested ace_bitslice

test.ml
@@ -1,9 +1,13 @@
+open Semantic_aes
 
+let rec to_nat n =
+  if n = 0 then O
+  else S (to_nat (n - 1))
 
 let rec gen_bin_list n =
   if 0 = n
   then []
-  else (if Random.int 2 = 0 then O else S O)::gen_bin_list (n - 1)
+  else (if Random.int 2 = 0 then Z.of_nat O else Z.of_nat (S O))::gen_bin_list (n - 1)
 
 let test_aes =
   let l = gen_bin_list (12 * 128) in
@@ -12,3 +16,11 @@ let test_aes =
 let () = match test_aes with
   | None -> print_endline "Failure AES"
   | Some _ -> print_endline "Success AES"
+
+let test_ace =
+  let l = gen_bin_list (2 * 5) in
+  prog_sem default_arch prog_ace_bs None [CoIR (DirV (to_nat 32), l, None)]
+
+let () = match test_ace with
+  | None -> print_endline "Failure ACE"
+  | Some _ -> print_endline "Success ACE"
