src/examples/ace_bitsliceTest.v
@@ -1,0 +1,189 @@
+
+Require Import ZArith String List.
+From Usuba Require Import arch utils usuba_AST usuba_ASTProp usuba_sem usuba_semProp ace_bitslice.
+Require Import Lia.
+
+Lemma node_f_soundness:
+    forall x,
+        exists v, eval_node default_arch node_f nil None (CoIR (DirV 32) (x::nil) None::nil)
+            = Some (CoIR (DirV 32) (v::nil) (Some (1::nil))::nil).
+Proof.
+    intro x.
+    unfold prog_sem.
+    cbn - [eval_expr].
+    unfold eval_expr, eval_var, eval_arith_expr.
+    cbn - [eval_shift].
+    unfold eval_shift, shift_wrapper, default_arch, IMPL_SHIFT.
+    pose (p := lrotate 32 (Pos.to_nat 5) x); fold p.
+    unfold Pos.to_nat; cbn.
+    eexists; reflexivity.
+Qed.
+
+Ltac simpl_1 iL Abs :=
+    let h := fresh "hd" in
+    destruct iL as [|h iL];
+    [> discriminate Abs | simpl in Abs].
+
+
+Ltac gen_notation_inner a :=
+    lazymatch a with
+    | match ?b with Some _ => _ | None => _ end => gen_notation_inner b
+    | _ => let H := fresh "H" in pose (H := a)
+    end.
+
+Ltac gen_notation :=
+    lazymatch goal with
+    | |- ?g <> None => gen_notation_inner g
+    end.
+
+
+Ltac simpl_util_inner a :=
+    lazymatch a with
+    | match ?b with Some _ => _ | None => _ end => simpl_util_inner b
+    | eval_node _ _ nil None (CoIR _ (?e::nil) _::_) =>
+        let v := fresh "v" in
+        destruct (node_f_soundness e) as [v ->]
+    | _ => let H := fresh "H" in pose (H := a)
+    end.
+
+Ltac simpl_util :=
+    lazymatch goal with
+    | |- exists v1 v2, ?g = _ => simpl_util_inner g
+    end.
+
+Lemma node_simeck_box_soundness:
+    forall iL, length iL = 3 ->
+        exists v1 v2,
+            eval_node default_arch node_simeck_box ((Id_s syntax.f, eval_node default_arch node_f nil)::nil) None (CoIR (DirV 32) iL None::nil)
+            = Some (CoIR (DirV 32) (v1::v2::nil) (Some (2::nil))::nil).
+Proof.
+    intros iL Hlength.
+    do 3 simpl_1 iL Hlength.
+    destruct iL; [> clear Hlength | discriminate Hlength].
+    cbn - [node_f].
+    unfold bind.
+    cbn - [eval_node].
+    unfold Pos.to_nat.
+    cbn - [eval_node].
+    destruct (node_f_soundness hd) as [v1 ->].
+    cbn - [eval_node].
+    unfold Pos.to_nat.
+    cbn - [eval_node].
+    unfold Pos.to_nat.
+    cbn - [eval_node].
+    simpl_util; cbn - [eval_node].
+    simpl_util; cbn - [eval_node].
+    simpl_util; cbn - [eval_node].
+    simpl_util; cbn - [eval_node].
+    simpl_util; cbn - [eval_node].
+    simpl_util; cbn - [eval_node].
+    simpl_util; cbn - [eval_node].
+    eexists; eexists.
+    reflexivity.
+Qed.
+
+Ltac simpl_util_inner' a :=
+    lazymatch a with
+    | match ?b with Some _ => _ | None => _ end => simpl_util_inner' b
+    | eval_node node_f _ nil None (CoIR _ (?e::nil) _::_) =>
+        let v := fresh "v" in
+        destruct (node_f_soundness e) as [v ->]
+    | eval_node _ node_simeck_box _ None (CoIR _ ?l _::_) =>
+        let v1 := fresh "v" in
+        let v2 := fresh "v" in
+        destruct (node_simeck_box_soundness l) as [v1 [v2 ->]]; [> auto | idtac]
+    | _ => let H := fresh "H" in pose (H := a)
+    end.
+
+Ltac simpl_util' :=
+    lazymatch goal with
+    | |- exists v1, ?g = _ /\ _ => simpl_util_inner' g
+    end.
+
+Lemma node_ACE_step_soundness:
+    forall iL, length iL = 16 ->
+        exists l,
+        eval_node default_arch node_ACE_step
+            ((Id_s simeck_box, eval_node default_arch node_simeck_box ((Id_s syntax.f, eval_node default_arch node_f nil)::nil))
+            :: (Id_s syntax.f, eval_node default_arch node_f nil)::nil)
+            None (CoIR (DirV 32) iL None::nil) = Some (CoIR (DirV 32) l None::nil)
+        /\ length l = 10.
+Proof.
+    intros iL Hlength.
+    do 16 simpl_1 iL Hlength.
+    destruct iL; [> clear Hlength | discriminate Hlength].
+    unfold eval_node.
+    cbn - [eval_node_inner eval_node].
+    unfold Pos.to_nat.
+    cbn - [eval_node_inner eval_node].
+    unfold eval_node_inner.
+    cbn - [eval_deq_list eval_node].
+    unfold Pos.to_nat; cbn - [eval_node].
+    simpl_util'; cbn - [eval_node].
+    unfold Pos.to_nat; cbn - [eval_node].
+    simpl_util'; cbn - [eval_node].
+    simpl_util'; cbn - [eval_node].
+    simpl_util'; cbn - [eval_node].
+    simpl_util'; cbn - [eval_node].
+    eexists; split.
+    + reflexivity.
+    + auto.
+Qed.
+
+Ltac simpl_util_inner'' a :=
+    lazymatch a with
+    | match ?b with Some _ => _ | None => _ end => simpl_util_inner'' b
+    | eval_node node_f _ nil None (CoIR _ (?e::nil) _::_) =>
+        let v := fresh "v" in
+        destruct (node_f_soundness e) as [v ->]
+    | eval_node _ node_simeck_box _ None (CoIR _ ?l _::_) =>
+        let v1 := fresh "v" in
+        let v2 := fresh "v" in
+        destruct (node_simeck_box_soundness l) as [v1 [v2 ->]]; [> auto | idtac]
+    | eval_node _ node_ACE_step _ None (CoIR _ ?l _::_) =>
+        let v := fresh "l" in
+        destruct (node_ACE_step_soundness l) as [v [-> Hlength]];
+        [> simpl; reflexivity | idtac];
+        do 10 simpl_1 v Hlength; destruct v;
+        [> clear Hlength | discriminate Hlength]
+    | _ => let H := fresh "H" in pose (H := a)
+    end.
+
+Ltac simpl_util2 :=
+    lazymatch goal with
+    | |- ?g <> None => simpl_util_inner'' g
+    end.
+
+Goal
+    forall iL, length iL = 10 ->
+    eval_node default_arch node_ACE (eval_prog default_arch (node_ACE_step::node_simeck_box::node_f::nil)) None (CoIR (DirV 32) iL None::nil) <> None.
+Proof.
+    intros iL Hlength;
+    do 10 simpl_1 iL Hlength; destruct iL; [> clear Hlength | discriminate Hlength].
+    unfold eval_node; cbn - [eval_deq_list eval_node].
+    unfold Pos.to_nat; cbn - [eval_deq_list eval_node].
+    cbn - [eval_node].
+    unfold bind.
+    cbn - [eval_node].
+    unfold Pos.to_nat; cbn - [eval_node].
+    simpl_util2.
+    unfold Pos.to_nat; cbn - [eval_node].
+    unfold Pos.to_nat; cbn - [eval_node].
+    simpl_util2; cbn - [eval_node].
+    simpl_util2; cbn - [eval_node].
+    simpl_util2; cbn - [eval_node].
+    simpl_util2; cbn - [eval_node].
+    simpl_util2; cbn - [eval_node].
+    simpl_util2; cbn - [eval_node].
+    simpl_util2; cbn - [eval_node].
+    simpl_util2; cbn - [eval_node].
+    simpl_util2; cbn - [eval_node].
+    simpl_util2; cbn - [eval_node].
+    simpl_util2; cbn - [eval_node].
+    simpl_util2; cbn - [eval_node].
+    simpl_util2; cbn - [eval_node].
+    simpl_util2; cbn - [eval_node].
+    simpl_util2; cbn - [eval_node].
+    discriminate.
+Qed.
+
