src/extract.v
@@ -3,7 +3,7 @@ Require Import ZArith.
 From Usuba Require Import usuba_AST collect clean
     usuba_sem arch aes ace_bitslice.
 Require Extraction.
-Require Import ExtrOcamlNativeString.
+Require Import ExtrOcamlNativeString ExtrOcamlZBigInt.
 
 Extraction Language OCaml.
 
@@ -12,4 +12,4 @@ Extract Inductive bool => bool [ true false ].
 Extract Inductive list => "list" [ "[]" "(::)" ]. 
 Extraction "usuba" clean_prog.
 
-Extraction "semantic_aes" prog_sem prog_aes default_arch.
+Extraction "semantic_aes" prog_sem prog_aes prog_ace_bs default_arch.
